theories/Dot/fundamental.v
@@ -19,18 +19,17 @@ Notation "Γ ⊨[ gφ  ] T1 , i <: T2 , j" := (wellMappedφ gφ -∗ step_indexe
 
 Section fundamental.
   Context `{!dlangG Σ} `{!SwapPropI Σ}.
-  Context `{hasStampTable: stampTable}.
 
-  Fixpoint fundamental_dm_typed Γ V l d T (HT: Γ |d V ⊢[ g ]{ l := d } : T) { struct HT }:
-    Γ |L V ⊨[ ⟦ getStampTable ⟧g ] { l := d } : T with
-  fundamental_dms_typed Γ V ds T (HT: Γ |ds V ⊢[ g ] ds : T) { struct HT }:
-    Γ |L V ⊨[ ⟦ getStampTable ⟧g ]ds ds : T with
-  fundamental_subtype Γ T1 i1 T2 i2 (HT: Γ ⊢ₜ[ g ] T1, i1 <: T2, i2) { struct HT }:
-    Γ ⊨[ ⟦ getStampTable ⟧g ] T1, i1 <: T2, i2 with
-  fundamental_typed Γ e T (HT: Γ ⊢ₜ[ g ] e : T) { struct HT }:
-    Γ ⊨[ ⟦ getStampTable ⟧g ] e : T with
-  fundamental_path_typed Γ p T i (HT : Γ ⊢ₚ[ g ] p : T, i) { struct HT }:
-    Γ ⊨[ ⟦ getStampTable ⟧g ]p p : T, i.
+  Fixpoint fundamental_dm_typed Γ g V l d T (HT: Γ |d V ⊢[ g ]{ l := d } : T) { struct HT }:
+    Γ |L V ⊨[ ⟦ g ⟧g ] { l := d } : T with
+  fundamental_dms_typed Γ g V ds T (HT: Γ |ds V ⊢[ g ] ds : T) { struct HT }:
+    Γ |L V ⊨[ ⟦ g ⟧g ]ds ds : T with
+  fundamental_subtype Γ g T1 i1 T2 i2 (HT: Γ ⊢ₜ[ g ] T1, i1 <: T2, i2) { struct HT }:
+    Γ ⊨[ ⟦ g ⟧g ] T1, i1 <: T2, i2 with
+  fundamental_typed Γ g e T (HT: Γ ⊢ₜ[ g ] e : T) { struct HT }:
+    Γ ⊨[ ⟦ g ⟧g ] e : T with
+  fundamental_path_typed Γ g p T i (HT : Γ ⊢ₚ[ g ] p : T, i) { struct HT }:
+    Γ ⊨[ ⟦ g ⟧g ]p p : T, i.
   Proof.
     - iIntros "#Hm"; induction HT.
       + iApply D_Typ_Abs; by [> iApply fundamental_subtype .. |
@@ -111,11 +110,11 @@ Proof.
   iIntros (??) "Hs"; iApply Hlog. by iApply transfer_empty.
 Qed.
 
-Corollary type_soundness_storeless e T `{!stampTable}:
+Corollary type_soundness_storeless e T g:
   [] ⊢ₜ[ g ] e : T → safe e.
 Proof.
   intros HsT.
-  apply: (adequacy_mapped_semtyping dlangΣ e getStampTable T); intros.
+  apply: (adequacy_mapped_semtyping dlangΣ e g T); intros.
   apply fundamental_typed, HsT.
 Qed.
 
